**Problem:**
We have an array `A` of integers, and an array `queries` of queries.

For the `i`-th query `val = queries[i][0], index = queries[i][1]`, we add val to `A[index]`. Then, the answer to the `i`-th query is the sum of the even values of `A`.

*(Here, the given `index = queries[i][1]` is a 0-based index, and each query permanently modifies the array `A`.)*

Return the answer to all queries. Your `answer` array should have `answer[i]` as the answer to the `i`-th query.

 

**Example 1:**

```
Input: A = [1,2,3,4], queries = [[1,0],[-3,1],[-4,0],[2,3]]
Output: [8,6,2,4]
Explanation: 
At the beginning, the array is [1,2,3,4].
After adding 1 to A[0], the array is [2,2,3,4], and the sum of even values is 2 + 2 + 4 = 8.
After adding -3 to A[1], the array is [2,-1,3,4], and the sum of even values is 2 + 4 = 6.
After adding -4 to A[0], the array is [-2,-1,3,4], and the sum of even values is -2 + 4 = 2.
After adding 2 to A[3], the array is [-2,-1,3,6], and the sum of even values is -2 + 6 = 4.
```

 

**Note:**

1. `1 <= A.length <= 10000`
2. `-10000 <= A[i] <= 10000`
3. `1 <= queries.length <= 10000`
4. `-10000 <= queries[i][0] <= 10000`
5. `0 <= queries[i][1] < A.length`
**My Solution:**
```
vector<int> sumEvenAfterQueries(vector<int>& A, vector<vector<int>>& queries) {
        int sum = 0;
        vector<int> result(queries.size());
        for (int i = 0; i < A.size(); i++) {
            if (A[i] % 2 == 0) {
                sum += A[i];
            }
        }
        for (int i = 0; i < queries.size(); i++) {
            int val = queries[i][0];
            int index = queries[i][1];
            if (A[index] % 2 == 0) {
                sum -= A[index];
            }
            A[index] += val;
            if (A[index] % 2 == 0) {
                sum += A[index];
            }
            result[i] = sum;
        }
        return result;
    }
```
Correctness:

We should first get the sum of even numbers in the array and when we get queries, we should decide whether we should change the sum.

Complexity:

Time: O(n)
Space: O(1)